ulib/FStar.Int.fst
@@ -453,10 +453,12 @@ let logand_pow2_minus_one #n a m =
 
 val logand_max: #n:pos{1 < n} -> a:int_t n{0 <= a} ->
   Lemma (0 <= logand a (max_int n) /\ a = logand a (max_int n))
+#push-options "--z3rlimit_factor 2"
 let logand_max #n a =
   sign_bit_positive a;
   sign_bit_positive #n (max_int n);
   nth_lemma a (logand a (max_int n))
+#pop-options
 
 (* Bitwise XOR operator *)
 val logxor_commutative: #n:pos -> a:int_t n -> b:int_t n ->
